CPO_domains_everywhere.v
@@ -1,0 +1,243 @@
+
+Require Import Coq.Setoids.Setoid.
+Require Import Coq.Classes.Morphisms.
+Require Import Coq.Arith.Arith_base.
+
+
+(***
+ *** Domains (which are just pre-orders with a fancy name)
+ ***)
+
+Class DomainOrder (A:Type) : Type :=
+  approx : relation A.
+
+(* Notation for approx *)
+Notation "x '<<<' y" := (approx x y) (at level 80, no associativity).
+
+Class Domain (A:Type) {DomainOrder:DomainOrder A} : Prop :=
+  {
+    domain_preorder :> PreOrder approx
+  }.
+
+(* For setoid_rewrite using approx *)
+Add Parametric Relation `{Domain} : A approx
+  reflexivity proved by PreOrder_Reflexive
+  transitivity proved by PreOrder_Transitive
+as Domain_morphism.
+
+(* The restriction of an approximation relation to an equivalence *)
+Definition approxEq `{DomainOrder} : relation A :=
+  fun a1 a2 => approx a1 a2 /\ approx a2 a1.
+
+(* Notation for approxEq *)
+Notation "m1 '==' m2" := (approxEq m1 m2) (at level 80, no associativity).
+
+(* approxEq is always an equivalence *)
+Instance approxEq_Equivalence `{Domain} : Equivalence approxEq.
+  constructor.
+  intro m; split; reflexivity.
+  intros m1 m2 H1; destruct H1; split; assumption.
+  intros m1 m2 m3 H1 H2; destruct H1; destruct H2; split; transitivity m2; assumption.
+Qed.
+
+(* For setoid_rewrite using approxEq *)
+Add Parametric Relation `{Domain} : A approxEq
+  reflexivity proved by Equivalence_Reflexive
+  symmetry proved by Equivalence_Symmetric
+  transitivity proved by Equivalence_Transitive
+as approxEq_morphism.
+
+(* For rewriting the arguments of approx using approxEq *)
+Instance proper_approxEq_approx `{Domain} : Proper (approxEq ==> approxEq ==> iff) approx.
+  intros x1 y1 eq1 x2 y2 eq2; destruct eq1; destruct eq2; split; intro.
+  transitivity x1; [ assumption | ]; transitivity x2; assumption.
+  transitivity y1; [ assumption | ]; transitivity y2; assumption.
+Qed.
+
+
+(***
+ *** Some useful domains
+ ***)
+
+(* Domains for pairs *)
+Instance Pair_DomainOrder A {_:DomainOrder A} B {_:DomainOrder B} :
+  DomainOrder (A*B) :=
+  fun p1 p2 => approx (fst p1) (fst p2) /\ approx (snd p1) (snd p2).
+
+Instance Pair_Domain A `{Domain A} B `{Domain B} : Domain (prod A B).
+  repeat constructor; try reflexivity; destruct H1; destruct H2.
+  transitivity (fst y); assumption.
+  transitivity (snd y); assumption.
+Qed.
+
+
+(***
+ *** Complete Partial Orders
+ ***
+ *** Technically, these are omega-complete preorders, since cpo_sup only deals
+ *** with countable chains and we drop antisymmetry.
+ ***)
+
+(* States that a is an upper bound of chain *)
+Definition upper_bound {A} (R: relation A) (chain: nat -> A) a :=
+  forall n, R (chain n) a.
+
+(* States that a is no greater than any upper bound of chain *)
+Definition below_upper_bounds {A} (R: relation A) (chain: nat -> A) a :=
+  forall a', upper_bound R chain a' -> R a a'.
+
+(* The supremum function, which works on any countable set of A's *)
+Class CPOSupremum (A:Type) {DomainOrder:DomainOrder A} : Type :=
+  cpo_sup : (nat -> A) -> A.
+
+(* The definition of a directed countable set *)
+Definition directed `{CPOSupremum} (chain: nat -> A) : Prop :=
+  forall n1 n2, exists n',
+    approx (chain n1) (chain n') /\ approx (chain n2) (chain n').
+
+(* (Omega)-CPO = preorder with least upper bounds of directed countable sets *)
+Class CPO (A:Type) {DomainOrder:DomainOrder A}
+      {CPOSupremum:@CPOSupremum A DomainOrder} : Prop :=
+  {
+    cpo_preorder :> Domain A;
+    cpo_sup_upper_bound :
+      forall chain, directed chain -> upper_bound approx chain (cpo_sup chain);
+    cpo_sup_least :
+      forall chain,
+        directed chain -> below_upper_bounds approx chain (cpo_sup chain)
+  }.
+
+(* Two supremums are equivalent iff the chains dominate each other *)
+Lemma supremums_equivalent `{CPO} chain1 chain2 :
+  directed chain1 -> directed chain2 ->
+  (forall n1, exists n2, approx (chain1 n1) (chain2 n2)) ->
+  (forall n2, exists n1, approx (chain2 n2) (chain1 n1)) ->
+  approxEq (cpo_sup chain1) (cpo_sup chain2).
+  intros; split; apply cpo_sup_least; try assumption; intro n.
+  destruct (H2 n) as [ n' ]; transitivity (chain2 n'); [ assumption | ].
+  apply cpo_sup_upper_bound; assumption.
+  destruct (H3 n) as [ n' ]; transitivity (chain1 n'); [ assumption | ].
+  apply cpo_sup_upper_bound; assumption.
+Qed.
+
+
+(***
+ *** Scott-Continuous Functions
+ ***)
+
+(* Scott-continuity = monotonicity + preservation of cpo_sup
+
+NOTE: We put monotonicity as part of the definition of Scott-continuity because
+we don't include antisymmetry in our definition of CPO, and the proof that
+Scott-continuity implies monotonicity requires a congruence closure step to
+prove that (f a2) = (f (cpo_sup (fun n => match n with | 0 => a1 | S _ => a2)))
+and this does not work when we only know that a2 is equivalent up to R to this
+supremum, not that it is equal. *)
+Definition scott_continuous `{CPO} (f : A -> A) : Prop :=
+  Proper (approx ==> approx) f /\
+  (forall chain,
+     directed chain ->
+     approxEq (f (cpo_sup chain)) (cpo_sup (fun n => f (chain n)))).
+
+
+(***
+ *** Pointed (omega-)CPOs
+ ***)
+
+(* The bottom of a PCPO *)
+Class PCPOBottom (A:Type) {DomainOrder:DomainOrder A} : Type :=
+  pcpo_bottom : A.
+
+(* PCPO = CPO + a bottom *)
+Class PCPO (A:Type) {DomainOrder:DomainOrder A}
+      {CPOSupremum:CPOSupremum A (DomainOrder:=DomainOrder)}
+      {PCPOBottom:PCPOBottom A (DomainOrder:=DomainOrder)} : Prop :=
+  {
+    pcpo_cpo :> CPO A (CPOSupremum:=CPOSupremum);
+    pcpo_least_element : forall a, approx pcpo_bottom a
+  }.
+
+
+(***
+ *** Every Scott-continuous function has a least fixed-point
+ ***)
+
+(* Fixed-points of f, modulo the symmetric closure of R *)
+Definition fixed_point `{DomainOrder} (f: A -> A) a :=
+  approxEq (f a) a.
+
+(* Least fixed-points of f, modulo the symmetric closure of R *)
+Definition least_fixed_point `{DomainOrder} (f: A -> A) a :=
+  fixed_point f a /\
+  forall a', fixed_point f a' -> approx a a'.
+
+(* Iterate a function n times *)
+Fixpoint iterate_f {A} n (f: A -> A) :=
+  match n with
+    | 0 => fun x => x
+    | S n' => fun x => f (iterate_f n' f x)
+  end.
+
+(* (f^n _|_) `R` (f^(n+1) _|_) for monotone f *)
+Lemma iterate_f_increases1 `{PCPO} n f :
+  Proper (approx ==> approx) f ->
+  approx (iterate_f n f pcpo_bottom) (iterate_f (S n) f pcpo_bottom).
+  intro mono; induction n.
+  apply pcpo_least_element.
+  unfold iterate_f; fold (@iterate_f A).
+  apply mono. assumption.
+Qed.
+
+(* Similar to above, but for arbitrary n1 <= n2 *)
+Lemma iterate_f_increases `{PCPO} n1 n2 f :
+  n1 <= n2 -> Proper (approx ==> approx) f ->
+  approx (iterate_f n1 f pcpo_bottom) (iterate_f n2 f pcpo_bottom).
+  intro l; induction l; intros.
+  reflexivity.
+  transitivity (iterate_f m f pcpo_bottom).
+  apply IHl; assumption.
+  apply iterate_f_increases1; assumption.
+Qed.
+
+(* Building the least fixed-point of a Scott-continuous function f *)
+Definition leastFP `{DomainOrder} {_:CPOSupremum A} {_:PCPOBottom A} f : A :=
+  cpo_sup (fun n => iterate_f n f pcpo_bottom).
+
+(* Proof that leastFP gives a fixed-point *)
+Lemma leastFP_correct `{PCPO} f :
+  scott_continuous f -> least_fixed_point f (leastFP f).
+  intro sc; destruct sc.
+
+  (* Helper lemma 1 *)
+  assert (directed (fun n : nat => iterate_f n f pcpo_bottom)).
+  intros n1 n2; exists (max n1 n2).
+  split; apply iterate_f_increases;
+    first [ assumption | apply Nat.le_max_l | apply Nat.le_max_r ].
+
+  (* Helper lemma 2 *)
+  assert (directed (fun n : nat => f (iterate_f n f pcpo_bottom))).
+  intros n1 n2; exists (max n1 n2).
+  unfold iterate_f; fold (@iterate_f A (S n1) f pcpo_bottom);
+  fold (@iterate_f A (S n2) f pcpo_bottom);
+  fold (@iterate_f A (S (max n1 n2)) f pcpo_bottom).
+  split; apply iterate_f_increases; try (apply le_n_S);
+    first [ assumption | apply Nat.le_max_l | apply Nat.le_max_r ].
+
+  split; unfold leastFP, fixed_point.
+
+  (* Proof that leastFP is a fixed-point *)
+  transitivity (cpo_sup (fun n => f (iterate_f n f pcpo_bottom))).
+  apply H1; assumption.
+  apply supremums_equivalent; try assumption; intro.
+  exists (S n1); reflexivity.
+  exists n2. apply iterate_f_increases1; assumption.
+
+  (* Proof that leastFP is a least fixed-point *)
+  intros fp is_fp.
+  apply cpo_sup_least; try assumption.
+  intro n; induction n.
+  apply pcpo_least_element.
+  transitivity (f fp).
+  apply H0; assumption.
+  destruct is_fp; assumption.
+Qed.
